src/ReactorModel/Objects/Reactor/Theorems/LawfulUpdate.lean
@@ -9,9 +9,29 @@ theorem UniqueIDs.updated [ReactorType.WellFounded α] {rtr₁ rtr₂ : α}
       |>.trans (Equivalent.from_lawfulUpdate u m₂).symm 
       |>.to_eq
 
+theorem LawfulMemUpdate.member₁ [ReactorType α] {rtr₁ rtr₂ : α}
+    (u : LawfulMemUpdate cpt i f rtr₁ rtr₂) : Member cpt i rtr₁ :=
+  sorry
+
+theorem LawfulMemUpdate.member₂ [ReactorType α] {rtr₁ rtr₂ : α}
+    (u : LawfulMemUpdate cpt i f rtr₁ rtr₂) : Member cpt i rtr₂ :=
+  sorry -- by u.member₁ and u.equiv
+
+theorem LawfulUpdate.ne_comm [ReactorType α] {rtr rtr₁ rtr₁' rtr₂ rtr₂' : α} 
+    (u₁ : LawfulUpdate cpt₁ i₁ f₁ rtr rtr₁) (u₂ : LawfulUpdate cpt₂ i₂ f₂ rtr₁ rtr₂) 
+    (u₁' : LawfulUpdate cpt₂ i₂ f₂ rtr rtr₁') (u₂' : LawfulUpdate cpt₁ i₁ f₁ rtr₁' rtr₂') 
+    (h : cpt₁ ≠ cpt₂ ∨ i₁ ≠ i₂) : rtr₂ = rtr₂' := by
+  cases u₁ <;> cases u₂' <;> cases u₂ <;> cases u₁'
+  case update.update.update.notMem =>
+    exact IsEmpty.elim ‹_› $ sorry
+    -- have := LawfulMemUpdate.member ‹_›  
+  all_goals sorry -- The only cases that should remain have matching kind on u₁&u₂' and u₂&u₁':
+            -- nnnn, nnuu, uunn, uuuu
+  -- Can you prove this without extensionality?
+
 open Updatable in
 theorem LawfulUpdatable.update_ne_comm [LawfulUpdatable α] {rtr : α} (h : cpt₁ ≠ cpt₂ ∨ i₁ ≠ i₂):
     update (update rtr cpt₁ i₁ f₁) cpt₂ i₂ f₂ = update (update rtr cpt₂ i₂ f₂) cpt₁ i₁ f₁ :=
-  sorry
-
+  LawfulUpdate.ne_comm (lawful ..) (lawful ..) (lawful ..) (lawful ..) h
+  
 end ReactorType
